# 28. Find the Index of the First Occurrence in a String (strStr)

## Question

Given two strings `needle` and `haystack`, return the index of the first occurrence of `needle` in `haystack`, or `-1` if `needle` is not part of `haystack`.&#x20;

**Example 1:**

<pre><code><strong>Input: haystack = "sadbutsad", needle = "sad"
</strong><strong>Output: 0
</strong><strong>Explanation: "sad" occurs at index 0 and 6.
</strong>The first occurrence is at index 0, so we return 0.
</code></pre>

**Example 2:**

<pre><code><strong>Input: haystack = "leetcode", needle = "leeto"
</strong><strong>Output: -1
</strong><strong>Explanation: "leeto" did not occur in "leetcode", so we return -1. 
</strong></code></pre>

**Constraints:**

* `1 <= haystack.length, needle.length <= 104`
* `haystack` and `needle` consist of only lowercase English characters.

## Solution

#### Java

```java
// sol: rolling hash
class Solution {
    private int base = 26;
    private int M = (int) 1e9 + 7;

    public int strStr(String haystack, String needle) {
        int m = haystack.length(), n = needle.length();
        if (m < n) {
            return -1;
        }
        int maxPow = 1;
        for (int i = 0; i < n; ++i) {
            maxPow = (maxPow * base) % M;
        }
        int hashNeedle = hash(needle);
        int hashStr = 0;
        for (int i = 0; i <= m - n; ++i) {
            if (i == 0) {
                hashStr = hash(haystack.substring(0, n));
            } else {
                hashStr = ((hashStr * base) % M - ((haystack.charAt(i - 1) - 'a') * maxPow) % M + (haystack.charAt(i + n - 1) - 'a') + M) % M;
            }
            if (hashStr == hashNeedle) {
                for (int j = 0; j < n; ++j) {
                    if (haystack.charAt(i + j) != needle.charAt(j)) {
                        break;
                    }
                    if (j == n - 1) {
                        return i;
                    }
                }
            }
        }
        return -1;
    }

    private int hash(String s) {
        int res = 0;
        long pow = 1;
        for (int i = s.length() - 1; i >= 0; --i) {
            res += ((s.charAt(i) - 'a') * pow) % M;
            pow = (pow * base) % M;
        }
        return res % M;
    }
}
```
